SkLean/DependentExamples.lean
@@ -14,6 +14,237 @@ abbrev S₀.{m, n, o} := ∀ (α : Type m) (β : Type n) (γ : Type o) (_x : α 
 def S₁ : S₀ := fun _α _β _γ x y z => x z (y z)
 
 /-
+## \\(M\\) combinator
 
+Normal \\(\Pi\\) typing:
+
+\\(\Pi (x : A), B x\\)
+
+`M` is basically the `S` combinator, but lhs is the body and rhs is the type signature. This allows higher-kinded type-expr composition. This makes the combinators fully dependently-typed.
+
+```
+def M : (∀ x : A, B x) := sorry
+mything : (?1 : Type → Type) := (?2 : Type → Type → Type)
+M mything ℕ := ?2 ℕ (?1 ℕ)
+```
+
+Notably, this allows us to fully eliminate binders in all types.
+We can simplify our type system using a notion of a "valid transition." `K`, `S`, and `M` are well-typed on their own. They are parametric over some types, respectively.
+Application is entirely what assigns meaning to these expressions. We **do not** need variables, substitution, or `∀` to express this.
 -/
+
+begin mutual
+
+inductive M where
+  | mk : M
+deriving Repr
+
+inductive S where
+  | mk : S
+deriving Repr
+
+inductive K where
+  | mk : K
+deriving Repr
+
+inductive Call where
+  | mk : Expr → Expr → Call
+deriving Repr
+
+inductive Expr where
+  | m    : M → Expr
+  | k    : K → Expr
+  | s    : S → Expr
+  | call : Call → Expr
+deriving Repr
+
+end
+
+mutual
+
+def sizeOfC (c : Call) : ℕ :=
+  match c with
+    | .mk lhs rhs => 2 + (sizeOf lhs) + (sizeOf rhs)
+
+def sizeOf (e : Expr) : ℕ :=
+  match e with
+    | .m _ => 1
+    | .s _ => 1
+    | .k _ => 1
+    | .call c => sizeOfC c
+
+end
+
+/-
+## DSL
+
+We make use of a small DSL for legibility.
+-/
+
+declare_syntax_cat skmexpr
+syntax "K"             : skmexpr
+syntax "S"             : skmexpr
+syntax "M"             : skmexpr
+syntax "(" skmexpr skmexpr ")" : skmexpr
+syntax ident           : skmexpr
+syntax "(" skmexpr ")" : skmexpr
+
+syntax " ⟪ " skmexpr " ⟫ " : term
+
+macro_rules
+  | `(⟪ K ⟫)                      => `(Expr.k .mk)
+  | `(⟪ S ⟫)                      => `(Expr.s .mk)
+  | `(⟪ M ⟫)                      => `(Expr.m .mk)
+  | `(⟪ $e:ident ⟫)               => `($e)
+  | `(⟪ ($e:skmexpr) ⟫)           => `(⟪$e⟫)
+  | `(⟪ ($e₁:skmexpr $e₂:skmexpr) ⟫) => `(Expr.call (.mk ⟪ $e₁ ⟫ ⟪ $e₂ ⟫))
+
+syntax "SKM[ " skmexpr " ] " : term
+
+macro_rules
+  | `(SKM[ $e:skmexpr ]) => `(⟪ $e ⟫)
+
+/-
+## Judgment Rules
+
+`K`, `M`, and `S` must be well-typed on their own. We need some expression that can represent the type of `K`. One option is the \\(\rightarrow\\) type constructor from the SLTC or System F. The typing of \\(S\\) and \\(K\\) are fairly obvious. However, the typing of \\(M\\) is not. It's not immediately clear that we need typing judgment rules for `K`, `M`, or `S` alone. There is no way to explicitly assign a type to `K`, `M`, or `S`. They just are. However, there are emergent rules for application. The typical rules for application in the SK combinator calculus are as follows:
+
+$$
+K : \alpha \rightarrow \beta \rightarrow \alpha \\\\
+S : (\alpha \rightarrow \beta \rightarrow \gamma) \rightarrow (\alpha \rightarrow \beta) \rightarrow \alpha \rightarrow \gamma \\\\
+M : hmm
+$$
+
+Typing rules quickly beome complicated. We would prefer to avoid binders in our type discipline. We can create an "emergent" typing based on function application.
+
+$$
+\frac{
+  \Gamma \vdash e_{1} : T
+}{
+  \Gamma \vdash K\ e_{1}\ e_{2} : T
+}
+$$
+$$
+\frac{
+  \Gamma \vdash f_{1}\ \text{arg}\ (f_{2}\ \text{arg}) : T)
+}{
+  \Gamma \vdash S\ f_{1}\ f_{2}\ \text{arg} : T
+}
+$$
+
+But what is the type of \\(K\\)? It's not really obvious. Clearly, we need some way to represent the type of \\(K\\) that avoids binders. Recall that:
+
+$$
+Kxy = x
+$$
+
+The type of \\(K\\) is typically \\(\alpha \rightarrow \beta \rightarrow \alpha\\). Its type is of the form of the \\(K\\) combinator. We can thus define a typing as such:
+
+$$
+K : K
+$$
+
+This typing is coherent under an evaluation rule for the \\(M\\) combinator:
+
+$$
+M\ (x : t)\ \text{arg} = x\ \text{arg}\ (t\ \text{arg}) \\\\
+M\ K\ \mathbb{N} = K\ \mathbb{N}\ (K\ \mathbb{N}) = \mathbb{N} \\\\
+M\ K\ K = K\ K\ (K\ K) = K \\\\
+\frac{
+  \Gamma \vdash e : ?, arg : t, (M\ e\ \text{arg} : t_{2})
+}{
+  \Gamma \vdash ? = t, e : t
+}
+$$
+-/
+
+mutual
+
+inductive is_eval_once : Call → Expr → Prop
+  | k x y     : is_eval_once (.mk SKM[(K x)] y) x
+  | s x y z   : is_eval_once (.mk SKM[((S x) y)] z) SKM[((x z) (y z))]
+  | m e t arg : valid_judgment e t → is_eval_once (.mk SKM[(M e)] arg) SKM[((e arg) (t arg))]
+  | rfl e₂    : (.call c) = e₂ → is_eval_once c e₂
+
+inductive beta_eq : SkExpr → SkExpr → Prop
+  | rfl                       : e₁ = e₂            → beta_eq e₁ e₂
+  | hard    e₁ (e₂ : Call) e₃ : is_eval_once e₂ e₃ → beta_eq e₁ e₃ → beta_eq e₁ (.call e₂)
+  | symm                      : beta_eq e₂ e₁ → beta_eq e₁ e₂
+  | trans                     : beta_eq e₁ e₂ → beta_eq e₂ e₃ → beta_eq e₁ e₃
+
+inductive valid_judgment : Expr → Expr → Prop
+  | k                    : valid_judgment SKM[K] SKM[K]
+  | s                    : valid_judgment SKM[S] SKM[S]
+  | m                    : valid_judgment SKM[M] SKM[M]
+  | call lhs rhs         : valid_judgment (.call (.mk lhs rhs)) SKM[((M lhs) rhs)]
+  | beta_eq e t₁ t₂      : valid_judgment e t₁ → beta_eq t₁ t₂ → valid_judgment e t₂
+
+end
+
+/-
+## Consistency
+
+In order to prove consistency of our type system, we need to demonstrate that no false statement can be constructed (thus, proving false). First, we will need to define `False` and `True`. `True` and `False` are typically encoded using the combinators as such (i.e., Church-encoding):
+
+$$
+T x y = x \\\\
+F x y = y
+$$
+-/
+
+def tre  := SKM[K]
+def flse := SKM[(S K)]
+
+/-
+We can prove consistency if we cannot construct an expression that occupies the type `flse`. A trivial case to attempt is the judgment `flse : flse`. If this holds from our judgment rules, we are cooked.
+-/
+
+lemma eval_once_imp_beta_eq : ∀ e e', is_eval_once e e'→ beta_eq (.call e) e' := by
+  intro e e' h_eval
+  apply beta_eq.symm
+  apply beta_eq.hard _ e e'
+  exact h_eval
+  simp [beta_eq.rfl]
+
+lemma call_self_not_beta_eq : ∀ e, ¬ is_eval_once (.mk e e) e := by
+  intro e h
+  cases h
+  case rfl h =>
+    cases e
+    case m m =>
+      simp_all
+    case k =>
+      simp_all
+    case s =>
+      simp_all
+    case call c =>
+      simp_all
+      apply_fun sizeOfC at h
+      simp [sizeOfC] at h
+      ring_nf at h
+      simp [_root_.sizeOf, sizeOfC] at h
+      linarith
+
+example : ¬(valid_judgment flse flse) := by
+  intro a
+  rw [flse] at *
+  cases a
+  case beta_eq e ht ht_beta_eq =>
+    cases ht
+    case call =>
+      cases ht_beta_eq
+      case rfl =>
+        simp_all
+      case hard e₃ h_beta_eq_e₃ h_t_e₃ =>
+        have h_eval : is_eval_once (.mk SKM[(M S)] SKM[K]) SKM[((S K) (S K))] := by
+          apply is_eval_once.m
+          simp [valid_judgment.s]
+        cases h_t_e₃
+        case rfl h =>
+          simp_all
+          apply eval_once_imp_beta_eq at h_eval
+          have h_eval_trans := beta_eq.trans (beta_eq.symm h_beta_eq_e₃) h_eval
+          
+          sorry
+    case beta_eq => sorry
 
