SkLean/Ast.lean
@@ -1,6 +1,7 @@
 /-
 # AST
 
+
 ## SK Polymorphic Typing
 
 I interpret the SK combinators as polymorphic functions of the form:
